driver/Clflags.ml
@@ -34,6 +34,7 @@ let option_finline_asm = ref false
 let option_mthumb = ref (Configuration.model = "armv7m")
 let option_Osize = ref false
 let option_finline = ref true
+let option_finline_functions_called_once = ref true
 let option_dprepro = ref false
 let option_dparse = ref false
 let option_dcmedium = ref false
